In SortingProb, renamed a lemma and added a lemma variant.
Work-in-progress on upper bound for merge sort.

work-in-progress/sorting/SortingUB.ec
@@ -19,7 +19,7 @@ timeout 2.  (* can increase *)
    the jth element (the answer is true or false); it can't ask
    questions about the values of the list elements themselves *)
 
-require import AllCore List IntDiv StdOrder IntMin FSetAux Perms Binomial.
+require import AllCore List IntDiv StdOrder IntMin FSetAux Perms Binomial WF.
 import IntOrder.
 
 require UpperBounds.       (* adversarial lower bounds framework *)
@@ -59,6 +59,253 @@ have not_tot_ord_xs : ! total_ordering xs.
 by rewrite f_bad.
 qed.
 (* end of realization *)
+
+require import AllCore List IntDiv StdOrder.
+import IntOrder.
+
+(* num : int -> int returns the worst case number of comparisons used
+   by merge sort when given a list of size n *)
+
+op num_wf_rec_def : (int, int) wf_rec_def =
+  fun (n : int,            (* input *)
+       f : int -> int) =>  (* for recursive calls on < natural numbers *)
+  if n <= 1  (* we only care about 1 <= n *)
+  then 0
+  else f (n %/ 2) + f (n %%/ 2) + n - 1.
+
+(* the actual recursive definition: *)
+
+op num : int -> int =
+  wf_recur
+  lt_nat           (* well-founded relation being used *)
+  0                (* element to be returned if recursive calls
+                      don't respect well-founded relation *)
+  num_wf_rec_def.  (* body of recursive definition *)
+
+lemma num_eq (n : int) :
+  1 <= n => num n = n * int_log 2 n - (2 ^ (int_log 2 n + 1) - n - 1).
+proof.
+move : n.
+apply (wf_ind lt_nat).
+apply wf_lt_nat.
+move => /= n IH ge1_n.
+case (n = 1) => [-> /= | ne1_n].
+rewrite /num wf_recur 1:wf_lt_nat /num_wf_rec_def /=.
+by rewrite int_log1_eq0 //= expr1.
+have ge2_n : 2 <= n by smt().
+rewrite /num wf_recur 1:wf_lt_nat /num_wf_rec_def.
+have -> /= : ! (n <= 1) by smt().
+have -> /= : lt_nat (n %/ 2) n by smt().
+have -> /= : lt_nat (n %%/ 2) n by smt().
+rewrite -/num.
+rewrite (IH (n %/ 2)) 1:/# 1:/#.
+rewrite (IH (n %%/ 2)) 1:/# 1:/#.
+rewrite int_log_div //=.
+have -> :
+  n %/ 2 * (int_log 2 n - 1) - (2 ^ int_log 2 n - n %/ 2 - 1) =
+  n %/ 2 * int_log 2 n - 2 ^ (int_log 2 n) + 1 by algebra.
+have -> :
+ n %%/ 2 * int_log 2 (n %%/ 2) -
+ (2 ^ (int_log 2 (n %%/ 2) + 1) - n %%/ 2 - 1) =
+ n %%/ 2 * int_log 2 (n %%/ 2) -
+ 2 ^ (int_log 2 (n %%/ 2) + 1) + n %%/ 2 + 1 by algebra.
+have -> :
+  n * int_log 2 n - (2 ^ (int_log 2 n + 1) - n - 1) =
+  n * int_log 2 n - 2 ^ (int_log 2 n + 1) + 1 + n by algebra.
+have -> :
+  n %/ 2 * int_log 2 n - 2 ^ int_log 2 n + 1 +
+  (n %%/ 2 * int_log 2 (n %%/ 2) -
+   2 ^ (int_log 2 (n %%/ 2) + 1) + n %%/ 2 + 1) +
+  n - 1 =
+  n %/ 2 * int_log 2 n - 2 ^ int_log 2 n +
+  n %%/ 2 * int_log 2 (n %%/ 2) - 2 ^ (int_log 2 (n %%/ 2) + 1)
+  + n %%/ 2 + 1 + n by algebra.
+rewrite -subr_eq addrK.
+rewrite -subr_eq addrK.
+have [lt | eq] :
+  n < 2 ^ (int_log 2 n + 1) - 1 \/ n = 2 ^ (int_log 2 n + 1) - 1.
+  smt(int_log_ub_lt).
+rewrite int_log2_divup_min1 //=.
+have -> :
+  n %/ 2 * int_log 2 n - 2 ^ int_log 2 n +
+  n %%/ 2 * (int_log 2 n - 1) - 2 ^ int_log 2 n + n %%/ 2 =
+  n %/ 2 * int_log 2 n + n %%/ 2 * int_log 2 n -
+  (2 ^ int_log 2 n + 2 ^ int_log 2 n) by algebra.
+by rewrite -mul2l -exprS 1:int_log_ge0 // -subr_eq addrK -mulrDl
+           -div2_plus_div2up_eq.
+rewrite int_log2_divup_eq //.
+have -> :
+  n %/ 2 * int_log 2 n - 2 ^ int_log 2 n + n %%/ 2 * int_log 2 n -
+  2 ^ (int_log 2 n + 1) + n %%/ 2 =
+  (n %/ 2 + n %%/ 2) * int_log 2 n + n %%/ 2
+  - 2 ^ int_log 2 n - 2 ^ (int_log 2 n + 1) by algebra.
+rewrite -subr_eq addrK -div2_plus_div2up_eq -addrA.
+have -> // : n %%/ 2 - 2 ^ int_log 2 n = 0.
+rewrite subr_eq /= int_div_up2_odd 1:eq /=.
+by rewrite odd_iff_plus1_even /= exprS 1:int_log_ge0 // dvdz_mulr.
+by rewrite {1}eq /= exprS 1:int_log_ge0 // mulKz.
+qed.
+
+lemma num_le (n : int) :
+  1 <= n => num n <= n * int_log 2 n.
+proof.
+move => ge1_n.
+rewrite num_eq // ler_subl_addr ler_addl.
+smt(int_log_ub_lt).
+qed.
+
+op merge (cmp : 'a -> 'a -> bool, xs ys : 'a list) : 'a list =
+  with xs = [],      ys = []      => []
+  with xs = [],      ys = _ :: _  => ys
+  with xs = _ :: _,  ys = []      => xs
+  with xs = u :: us, ys = v :: vs =>
+    if cmp u v
+    then u :: merge cmp us ys
+    else v :: merge cmp xs vs.
+
+lemma cmp_head_merge (cmp : 'a -> 'a -> bool, n : 'a, xs ys : 'a list) :
+  cmp n (head n xs) => cmp n (head n ys) =>
+  cmp n (head n (merge cmp xs ys)).
+proof.
+case xs => [| u us].
+by case ys.
+case ys => [// | v vs /=].
+by case (cmp u v).
+qed.
+
+lemma merge_sorted (e : 'a -> 'a -> bool, xs ys : 'a list) :
+  (forall (a : 'a), e a a) =>
+  (forall (a b : 'a), e a b \/ e b a) =>
+  sorted e xs => sorted e ys =>
+  sorted e (merge e xs ys).
+proof.
+move => refl_e tot_e; move : ys.
+elim xs => [| u us IH_outer].
+by case.
+elim => [// | v vs /= IH_inner path_u_us path_v_vs].
+case (e u v) => [e_u_v | not_e_u_v].
+rewrite (pathP u); right; split => [| /=].
+by rewrite cmp_head_merge cmp_head_path_same_def.
+by rewrite IH_outer (path_sorted _ u).
+rewrite (pathP v); right; split => [| /=].
+rewrite cmp_head_merge cmp_head_path_same_def //= path_u_us /= 1:/#.
+by rewrite IH_inner // (path_sorted _ v).
+qed.
+
+type term = [
+  | Sort  of int list  (* list is nonempty *)
+  | List  of int list
+  | Cons  of int & term
+  | Merge of term & term
+  | Cond  of int & int & term & term
+].
+
+op deft : term = List [].
+
+op repr (cmp : int -> int -> bool, t : term) : int list =
+  with t = Sort xs      => sort cmp xs
+  with t = List xs      => xs
+  with t = Cons i u     => i :: repr cmp u
+  with t = Merge u v    => merge cmp (repr cmp u) (repr cmp v)
+  with t = Cond i j u v =>
+    if cmp i j then repr cmp u else repr cmp v.
+
+op is_list (t : term) : bool =
+  with t = Sort xs      => false
+  with t = List xs      => true
+  with t = Cons i u     => false
+  with t = Merge u v    => false
+  with t = Cond i j u v => false.
+
+op of_list (t : term) : int list =
+  with t = Sort xs      => []
+  with t = List xs      => xs
+  with t = Cons i u     => []
+  with t = Merge u v    => []
+  with t = Cond i j u v => [].
+
+type step = [
+  | Stuck
+  | Step    of term
+  | Compare of int & int
+].
+
+op is_step (s : step) : bool =
+  with s = Stuck       => false
+  with s = Step t      => true
+  with s = Compare i j => false.
+
+op of_step (s : step) : term =
+  with s = Stuck       => deft
+  with s = Step t      => t
+  with s = Compare i j => deft.
+
+op is_compare (s : step) : bool =
+  with s = Stuck       => false
+  with s = Step t      => false
+  with s = Compare i j => true.
+
+op of_compare (s : step) : int * int =
+  with s = Stuck       => (0, 0)
+  with s = Step t      => (0, 0)
+  with s = Compare i j => (i, j).
+
+op step (t : term) : step =
+  with t = Sort xs =>
+    let mid = size xs %/ 2 in
+    Step
+    (Merge (Sort (take mid xs))  (* size: size xs %/ 2 *)
+    (Sort (drop mid xs)))        (* size: size xs %%/ 2 *)
+  with t = List xs => Stuck
+  with t = Cons n u =>
+    let u' = step u in
+    if is_step u'
+      then Step (Cons n (of_step u'))
+    else if is_compare u'
+      then u'
+    else if is_list u
+      then Step (List (n :: of_list u))
+    else Stuck
+  with t = Merge u v =>
+    let u' = step u in
+    if is_step u'
+      then Step (Merge (of_step u') v)
+    else if is_compare u'
+      then u'
+    else let v' = step v in
+         if is_step v'
+           then Step (Merge u (of_step v'))
+         else if is_compare v'
+           then v'
+         else if is_list u /\ is_list v
+           then if of_list u = []
+                  then Step v
+                else if of_list v = []
+                  then Step u
+                else let i = head 0 (of_list u) in
+                     let ms = behead (of_list u) in
+                     let j = head 0 (of_list v) in
+                     let ns = behead (of_list v) in
+                     Step (Cond i j
+                           (Cons i (Merge (List ms) v))
+                           (Cons j (Merge u (List ns))))
+         else Stuck
+  with t = Cond i j u v => Compare i j.
+
+op answer (t : term, b : bool) : term option =
+  with t = Sort xs => None
+  with t = List xs => None
+  with t = Cons n u =>
+    let u' = answer t b in
+    if u' = None then None else Some (Cons n (oget u'))
+  with t = Merge u v =>
+    let u' = answer u b in
+    if u' <> None
+    then Some (Merge (oget u') v)
+    else let v' = answer v b in
+         if v' = None then None else Some (Merge u (oget v'))
+  with t = Cond i j u v =>
+    if b then Some u else Some v.
 
 (* here is our algorithm: *)
 
